PORTING.md
@@ -192,7 +192,7 @@ Some porting tasks will require other tasks as dependencies, the GitHub issues p
 - [ ] `lib/proph_map.v`
 - [ ] `lib/saved_prop.v`
 - [ ] `lib/token.v`
-- [ ] `lib/wsat.v`
+- [x] `lib/wsat.v`
 
 ## BI
 
